theories/Runtime.v
@@ -1,0 +1,478 @@
+(** * Operational Semantics of Pat *)
+
+From MailboxTypes Require Export Environment.
+From MailboxTypes Require Export Syntax.
+From MailboxTypes Require Import Util.
+From MailboxTypes Require Import TypingRules.
+From MailboxTypes Require Import Substitution.
+
+From Stdlib Require Import ListSet.
+From Stdlib Require Import PeanoNat.
+
+Generalizable All Variables.
+
+Section runtime_def.
+  Context `{M : IMessage Message}.
+  Context `{D : IDefinitionName DefinitionName}.
+
+  (**
+    A stack is a simply a list of terms. Due to the usage of deBruijn indices
+    we don't include variable names in frames.
+    We will always replace variable 0.
+  *)
+  Definition Stack := list Term.
+
+  Inductive Configuration : Type :=
+    | ConfConf : Term -> Stack -> Configuration
+    | ConfMessage : VarName -> Message -> Value -> Configuration
+    | ConfParallel : Configuration -> Configuration -> Configuration
+    | ConfRestr : Configuration -> Configuration.
+
+  Fixpoint lower_conf (i : VarName) (c : Configuration) : Configuration :=
+    match c with
+    | ConfConf t s => ConfConf (lower i t) s
+    | ConfMessage x m v => ConfMessage (lower_Var i x) m (lower_Value i v)
+    | ConfParallel c1 c2 => ConfParallel (lower_conf i c1) (lower_conf i c2)
+    | ConfRestr c => ConfRestr (lower_conf (S i) c)
+    end.
+
+  Fixpoint exchange_conf (i : VarName) (c : Configuration) : Configuration :=
+    match c with
+    | ConfConf t s => ConfConf (exchange i t) s
+    | ConfMessage x m v => ConfMessage (exchange_Var i x) m (exchange_Value i v)
+| ConfParallel c1 c2 => ConfParallel (exchange_conf i c1) (exchange_conf i c2)
+    | ConfRestr c => ConfRestr (exchange_conf (S i) c)
+    end.
+
+  Fixpoint FV_conf (c : Configuration) : set nat :=
+    match c with
+    | ConfConf t s => FV t
+    | ConfMessage x m v =>
+        set_union Nat.eq_dec [x] (FV_val v)
+    | ConfParallel c1 c2 =>
+        set_union Nat.eq_dec (FV_conf c1) (FV_conf c2)
+    | ConfRestr c =>
+        (downShift 1 (set_remove Nat.eq_dec 0 (FV_conf c)))
+    end.
+
+  Inductive StructCongr : Configuration -> Configuration -> Prop :=
+    | CongrParSym : forall c d, StructCongr (ConfParallel c d) (ConfParallel d c)
+    | CongrAssoc : forall c d e,
+        StructCongr (ConfParallel c (ConfParallel d e)) (ConfParallel (ConfParallel c d) e)
+    | CongrRestrComm : forall c,
+        StructCongr (ConfRestr (ConfRestr c)) (ConfRestr (ConfRestr (exchange_conf 0 c)))
+    | CongrRestrExt : forall c d,
+        ~ In 0 (FV_conf d) ->
+        StructCongr (ConfRestr (ConfParallel c d)) (ConfParallel (ConfRestr c) (lower_conf 0 d))
+    | CongrRefl : forall c, StructCongr c c
+    | CongrSym : forall c d, StructCongr c d -> StructCongr d c
+    | CongrTrasn : forall c d e, StructCongr c d -> StructCongr d e -> StructCongr c e.
+
+  Inductive Step (prog : Prog) : Configuration -> Configuration -> Prop :=
+    | stepLet : forall t1 t2 stack,
+        Step prog (ConfConf (TLet t1 t2) stack) (ConfConf t1 (t2 :: stack))
+    | stepReturn : forall (v : Value) t stack,
+        Step prog (ConfConf (TValue v) (t :: stack)) (ConfConf (subst v 0 t) stack)
+    | stepApp : forall v stack definition bodyType argumentType t,
+        definitions prog definition = (FunDef definition argumentType bodyType t) ->
+        Step prog (ConfConf (TApp definition v) stack) (ConfConf (subst v 0 t) stack)
+    | stepNew : forall stack,
+        Step prog (ConfConf TNew stack) (ConfRestr (ConfConf (TValue (ValueVar 0)) stack))
+    | stepSend : forall stack x m v,
+        Step prog (ConfConf (TSend (ValueVar x) m v) stack)
+                  (ConfParallel (ConfConf (TValue (ValueUnit)) stack) (ConfMessage x m v))
+    | stepSpawn : forall stack t,
+        Step prog (ConfConf (TSpawn t) stack)
+                  (ConfParallel (ConfConf (TValue (ValueUnit)) stack) (ConfConf t []))
+    | stepFree : forall stack e guards t,
+        Exists (fun g => g = GFree t) guards ->
+        Step prog (ConfRestr (ConfConf (TGuard (ValueVar 0) e guards) stack))
+        (ConfConf t stack)
+    | stepReceive : forall stack e guards x m v t,
+        Exists (fun g => g = GReceive m t) guards ->
+        Step prog (ConfParallel (ConfConf (TGuard (ValueVar x) e guards) stack) (ConfMessage x m v))
+        (ConfConf ((subst v 0) (subst (ValueVar x) 0 t)) stack)
+    | stepNu : forall c d,
+        Step prog c d ->
+        Step prog (ConfRestr c) (ConfRestr d)
+    | stepPar : forall c c' d,
+        Step prog c c' ->
+        Step prog (ConfParallel c d) (ConfParallel c' d)
+    | stepStruct : forall c c' d d',
+        StructCongr c c' ->
+        StructCongr d' d ->
+        Step prog c' d' ->
+        Step prog c d.
+
+  Definition RuntimeEnv := env TType.
+
+  Inductive RuntimeEnvironmentCombination : RuntimeEnv -> RuntimeEnv -> RuntimeEnv -> Prop :=
+      RuntimeEnvCombEmpty : RuntimeEnvironmentCombination nil nil nil
+    (* Special constructor for our representation of environments *)
+    | RuntimeEnvCombNone : forall env1 env2 env,
+        RuntimeEnvironmentCombination env1 env2 env ->
+        RuntimeEnvironmentCombination (None :: env1) (None :: env2) (None :: env)
+    | RuntimeEnvCombLeft : forall env1 env2 env T,
+        RuntimeEnvironmentCombination env1 env2 env ->
+        RuntimeEnvironmentCombination (Some T :: env1) (None :: env2) (Some T :: env)
+    | EnvCombRight : forall env1 env2 env T,
+        RuntimeEnvironmentCombination env1 env2 env ->
+        RuntimeEnvironmentCombination (None :: env1) (Some T :: env2) (Some T :: env)
+    | EnvCombBoth : forall T env1 env2 env T1 T2,
+        RuntimeEnvironmentCombination env1 env2 env ->
+        T1 ⊞ T2 ~= T ->
+        RuntimeEnvironmentCombination (Some T1 :: env1) (Some T2 :: env2) (Some T :: env).
+
+  Inductive RuntimeSubtype : TType -> TType -> Prop :=
+      SubtypeBase : forall c, RuntimeSubtype (TTBase c) (TTBase c)
+    | SubtypeInput : forall e f,
+        MPInclusion e f -> RuntimeSubtype (TTMailbox (MTInput e)) (TTMailbox (MTInput f))
+    | SubtypeOutput : forall e f,
+        MPInclusion f e -> RuntimeSubtype (TTMailbox (MTOutput e)) (TTMailbox (MTOutput f)).
+
+  Definition ReliableType (T : TType) : Prop :=
+    ~ (RuntimeSubtype T (TTMailbox (? 𝟘))).
+
+  Definition ReliableEnv : RuntimeEnv -> Prop :=
+    ForallMaybe ReliableType.
+
+  Inductive RuntimeEnvironmentSubtype : RuntimeEnv -> RuntimeEnv -> Prop :=
+    | EnvSubtypeNone : forall env1 env2,
+        RuntimeEnvironmentSubtype env1 env2 ->
+        RuntimeEnvironmentSubtype (None :: env1) (None :: env2)
+    | EnvSubtypeDrop : forall env1 env2 T,
+        RuntimeEnvironmentSubtype env1 env2 ->
+        RuntimeEnvironmentSubtype (Some T :: env1) (None :: env2)
+    | EnvSubtypeSub : forall env1 env2 T1 T2,
+        RuntimeSubtype T1 T2 ->
+        RuntimeEnvironmentSubtype env1 env2 ->
+        RuntimeEnvironmentSubtype (Some T1 :: env1) (Some T2 :: env2)
+    | EnvSubtypeTrans : forall env1 env2 env3,
+        RuntimeEnvironmentSubtype env1 env2 ->
+        RuntimeEnvironmentSubtype env2 env3 ->
+        RuntimeEnvironmentSubtype env1 env3
+    | EnvSubtypeRefl : forall env, RuntimeEnvironmentSubtype env env.
+
+  Inductive WellTypedConfig (prog : Prog) : RuntimeEnv -> Configuration -> Prop :=
+    | NU : forall env c,
+        WellTypedConfig prog (Some (TTMailbox (? 𝟙)) :: env) c ->
+        WellTypedConfig prog env (ConfRestr c)
+    | PAR : forall env1 env2 env c d,
+        WellTypedConfig prog env1 c ->
+        WellTypedConfig prog env2 d ->
+        RuntimeEnvironmentCombination env1 env2 env ->
+        WellTypedConfig prog env (ConfParallel c d)
+    | MESSAGE : forall env v x m T,
+        WellTypedTerm prog (map_maybe secondType env) (TValue v) T ->
+        T ≤ ⌈ signature prog m ⌉ ->
+        WellTypedConfig prog (insert x (TTMailbox (! « m »)) env) (ConfMessage x m v)
+    | THREAD : forall env1 env2 env t T stack,
+        env1 ▷ₑ env2 ~= (map_maybe returnType env) ->
+        WellTypedTerm prog env1 t T ->
+        WellTypedFrame prog env2 T stack ->
+        WellTypedConfig prog env (ConfConf t stack)
+    | SUBS : forall env env' c,
+        RuntimeEnvironmentSubtype env env' ->
+        WellTypedConfig prog env' c ->
+        WellTypedConfig prog env c
+  with WellTypedFrame (prog : Prog) : Env -> TUsage -> Stack -> Prop :=
+    | EMPTY : forall T, WellTypedFrame prog [] T []
+    | CONS : forall env1 env2 env t T1 T2 stack,
+        WellTypedTerm prog (Some T1 :: env1) t T2 ->
+        ReturnableType T2 ->
+        WellTypedFrame prog env2 T2 stack ->
+        env1 ▷ₑ env2 ~= env ->
+        WellTypedFrame prog env T1 (t :: stack).
+
+End runtime_def.
+
+Notation "Env1 ⨝ₑ Env2 ~= Env" := (RuntimeEnvironmentCombination Env1 Env2 Env) (at level 80) : environment_scope.
+
+Section runtime_props.
+  Context `{M : IMessage Message}.
+  Context `{D : IDefinitionName DefinitionName}.
+
+  Lemma RuntimeSubtype_refl : forall T, RuntimeSubtype T T.
+  Proof.
+    destruct T; try destruct m; try constructor; apply MPInclusion_refl.
+  Qed.
+
+  Lemma RuntimeEnvironmentSubtype_refl : forall env, RuntimeEnvironmentSubtype env env.
+  Proof.
+    destruct env; constructor.
+  Qed.
+
+  Lemma RuntimeEnvironmentCombination_comm : forall env1 env2 env3,
+    env1 ⨝ₑ env2 ~= env3 -> env2 ⨝ₑ env1 ~= env3.
+  Proof.
+    intros * Comb.
+    induction Comb; try constructor; try apply IHComb.
+    now apply TypeCombination_comm.
+  Qed.
+
+  Lemma RuntimeEnvironmentCombination_assoc : forall env1 env2 env3 env2' env,
+    env1 ⨝ₑ env2' ~= env ->
+    env2 ⨝ₑ env3 ~= env2' ->
+    exists env1', env1' ⨝ₑ env3 ~= env /\ env1 ⨝ₑ env2 ~= env1'.
+  Proof.
+  Admitted.
+
+  Lemma RuntimeEnvironmentCombination_Subtype_right : forall env1 env2 env2' env,
+    env1 ⨝ₑ env2 ~= env ->
+    RuntimeEnvironmentSubtype env2 env2' ->
+    exists env', env1 ⨝ₑ env2' ~= env' /\ RuntimeEnvironmentSubtype env env'.
+  Proof.
+  Admitted.
+
+  Lemma RuntimeEnvironmentCombination_Subtype : forall env1 env2 env env',
+    env1 ⨝ₑ env2 ~= env ->
+    RuntimeEnvironmentSubtype env env' ->
+    exists env1' env2',
+      env1' ⨝ₑ env2' ~= env' /\
+      RuntimeEnvironmentSubtype env1 env1' /\
+      RuntimeEnvironmentSubtype env2 env2'.
+  Proof.
+  Admitted.
+
+  Lemma WellTypedConfig_exchange : forall x prog T c env,
+    WellTypedConfig prog (insert x T (insert x T env)) c ->
+    WellTypedConfig prog (insert x T (insert x T env)) (exchange_conf x c).
+  Proof.
+    intros * WT.
+    remember (insert x T (insert x T env)) as E.
+    revert x env T HeqE.
+    induction WT; intros; inversion HeqE; subst; simpl in *.
+    - assert (Eq : Some (TTMailbox (? 𝟙)) :: insert x T (insert x T env0) = insert (S x) T (insert (S x) T (Some (TTMailbox (? 𝟙)) :: env0))).
+      {
+        repeat rewrite raw_insert_successor.
+        now repeat rewrite lookup_zero.
+      }
+      generalize (IHWT (S x) (Some (TTMailbox (? 𝟙)) :: env0) T Eq).
+      intros WT'.
+      now constructor.
+    - econstructor.
+      + eapply IHWT1. admit.
+      + admit.
+      + admit.
+    - admit.
+    - admit.
+    - admit.
+  Admitted.
+
+  Lemma WellTypedConfig_PAR_inv : forall env c1 c2 prog,
+    WellTypedConfig prog env (ConfParallel c1 c2) ->
+    exists env1 env2,
+      RuntimeEnvironmentCombination env1 env2 env /\
+      WellTypedConfig prog env1 c1 /\ WellTypedConfig prog env2 c2.
+  Proof.
+    intros * WT.
+    remember (ConfParallel c1 c2) as C.
+    revert c1 c2 HeqC.
+    induction WT; intros; inversion HeqC; subst.
+    - now exists env1, env2.
+    - generalize (IHWT _ _ eq_refl).
+      intros [env1 [env2 [Comb [WT1 WT2]]]].
+      eapply RuntimeEnvironmentCombination_Subtype with (env' := env) in Comb.
+  Admitted.
+
+  Lemma WellTypedConfig_lower : forall x c env prog,
+    ~ In x (FV_conf c) ->
+    WellTypedConfig prog (repeat None (S x) ++ env) c ->
+    WellTypedConfig prog env (lower_conf x c).
+  Proof.
+    induction x; intros * In WT; simpl in *.
+    - induction c; simpl in *.
+      + admit.
+      + admit.
+      + eapply PAR.
+        * apply IHc1.
+          -- intros In'.
+  Admitted.
+
+
+  (*Lemma WellTypedConfig_lower : forall c env prog,*)
+  (*  ~ In 0 (FV_conf c) ->*)
+  (*  WellTypedConfig prog (None :: env) c ->*)
+  (*  WellTypedConfig prog env (lower_conf 0 c).*)
+  (*Proof.*)
+  (*  intros * In WT.*)
+  (*  remember (None :: env) as E.*)
+  (*  revert env HeqE.*)
+  (*  induction WT; intros; inversion HeqE; subst; simpl in *.*)
+  (*  - apply NU.*)
+  (**)
+  (*  induction c; intros * In WT; simpl in *.*)
+  (*  - admit.*)
+  (*  - inversion WT; subst.*)
+  (**)
+  (**)
+  (*  intros * WT.*)
+  (**)
+  (*  (*remember (None :: env) as E.*)*)
+  (*  (*revert env HeqE.*)*)
+  (*  (*induction WT; intros; inversion HeqE; subst.*)*)
+  (*  induction WT.*)
+  (*  - simpl in *.*)
+  (*    apply NU.*)
+
+  (*Lemma WellTypedConfig_lower : forall x c env prog,*)
+  (*  WellTypedConfig prog (raw_insert (S x) None env) c ->*)
+  (*  WellTypedConfig prog env (lower_conf x c).*)
+  (*Proof.*)
+  (*  intros x c.*)
+  (*  revert x.*)
+  (*  induction c; intros * WT; simpl in *.*)
+  (*  - rewrite raw_insert_successor in WT.*)
+  (*    destruct env.*)
+  (*    + rewrite lookup_nil in WT; simpl in *.*)
+  (*      admit.*)
+  (*    + admit.*)
+  (*  - eapply MESSAGE.*)
+
+
+  Lemma preservation_equiv : forall prog env c d,
+    WellTypedConfig prog env c ->
+    StructCongr c d ->
+    WellTypedConfig prog env d.
+  Proof.
+    intros * WTc Congr.
+    revert env WTc.
+    induction Congr; intros.
+    - remember (ConfParallel c d) as C.
+      revert c d HeqC.
+      induction WTc; intros; inversion HeqC; subst.
+      + eapply PAR; try eassumption.
+        now apply RuntimeEnvironmentCombination_comm.
+      + eapply SUBS; try eassumption.
+        now apply IHWTc.
+    - remember (ConfParallel c (ConfParallel d e)) as C.
+      revert c d e HeqC.
+      induction WTc; intros; inversion HeqC; subst.
+      + remember (ConfParallel d0 e) as E'.
+        revert env d0 e HeqE' H.
+        clear IHWTc1 IHWTc2.
+        induction WTc2; intros; inversion HeqE'; subst.
+        * generalize (RuntimeEnvironmentCombination_assoc _ _ _ _ _ H0 H).
+          intros [env' [Comb1 Comb2]].
+          eapply PAR; try eapply PAR; eassumption.
+        * generalize (RuntimeEnvironmentCombination_Subtype_right _ _ env' _ H0 H).
+          intros [env'' [Comb' Sub']].
+          eapply SUBS; try eassumption.
+          apply IHWTc2; auto.
+      + eapply SUBS; try eassumption.
+        now apply IHWTc.
+    - remember (ConfRestr (ConfRestr c)) as C.
+      revert c HeqC.
+      induction WTc; intros; inversion HeqC; subst.
+      + do 2 apply NU.
+        replace (Some (TTMailbox (? 𝟙)) :: Some (TTMailbox (? 𝟙)) :: env) with (insert 0 (TTMailbox (? 𝟙)) (insert 0 (TTMailbox (? 𝟙)) env)) by now repeat rewrite raw_insert_zero.
+        apply WellTypedConfig_exchange.
+        repeat rewrite raw_insert_zero.
+        clear IHWTc HeqC.
+        remember (ConfRestr c0) as C'.
+        revert c0 HeqC'.
+        induction WTc; intros; inversion HeqC'; subst.
+        * easy.
+        * eapply SUBS with (env' := Some (TTMailbox (? 𝟙)) :: env').
+          -- constructor.
+             apply RuntimeSubtype_refl.
+             assumption.
+          -- now apply IHWTc.
+      + eapply SUBS; try eassumption.
+        now apply IHWTc.
+    - remember (ConfRestr (ConfParallel c d)) as C.
+      revert c HeqC.
+      induction WTc; intros; inversion HeqC; subst.
+      + inversion WTc; subst.
+        * inversion H5; subst.
+          -- eapply PAR.
+             ++ apply NU. apply H2.
+             ++ admit.
+             ++ apply H6.
+          -- eapply PAR.
+             ++ apply NU. admit.
+             ++ admit.
+             ++ apply H6.
+          -- inversion H8; subst.
+             ++ eapply PAR.
+                ** apply NU.
+                   admit.
+                ** admit.
+                ** admit.
+             ++ admit.
+        * admit.
+
+
+      (**)
+      (**)
+      (*+ clear HeqC IHWTc.*)
+      (*  remember (Some (TTMailbox (? 𝟙)) :: env) as E.*)
+      (*  remember (ConfParallel c0 d) as C.*)
+      (*  revert env c0 HeqC HeqE.*)
+      (*  induction WTc; intros; inversion HeqC; subst.*)
+      (*  * inversion H0; subst.*)
+      (*    -- eapply PAR with (env1 := env3) (env2 := env4).*)
+      (*       ++ now apply NU.*)
+      (*       ++ admit.*)
+      (*       ++ eassumption.*)
+      (*    -- eapply PAR with (env2 := env4).*)
+      (*       ++ apply NU.*)
+      (*          eapply SUBS with (env' := None :: env3).*)
+      (*          ** constructor; apply RuntimeEnvironmentSubtype_refl.*)
+      (*          ** assumption.*)
+      (*       ++ admit.*)
+      (*       ++ eassumption.*)
+      (*    -- inversion H6; subst.*)
+      (*       ++ eapply PAR with (env1 := env3) (env2 := env4).*)
+      (*          ** apply NU. admit.*)
+      (*          ** admit.*)
+      (*          ** assumption.*)
+      (*       ++ eapply PAR with (env1 := env3) (env2 := env4).*)
+      (*          ** apply NU. admit.*)
+      (*          ** admit.*)
+      (*          ** assumption.*)
+      (*  * *)
+      (**)
+      (*    clear IHWTc H1.*)
+      (*    remember (Some (TTMailbox (? 𝟙)) :: env0) as E.*)
+      (*    remember (ConfParallel c0 d) as C.*)
+      (*    revert env0 c0 HeqC HeqE.*)
+      (*    induction WTc; intros; inversion HeqC; subst.*)
+      (*    -- eapply PAR.*)
+
+      + eapply SUBS; try eassumption.
+        now apply IHWTc.
+  Admitted.
+
+  Theorem preservation : forall prog env c d,
+    WellTypedProgram prog ->
+    ReliableEnv env ->
+    WellTypedConfig prog env c ->
+    Step prog c d ->
+    WellTypedConfig prog env d.
+  Proof.
+    intros * WTP Reliable WT Step.
+    revert env Reliable WT.
+    induction Step; intros.
+    - inversion WT; subst.
+      + inversion H3; subst.
+        * generalize (EnvironmentCombination_assoc).
+          econstructor.
+          -- admit.
+          -- apply H6.
+          --
+
+
+    induction WT; intros * Reliable Step.
+    - admit.
+    - inversion Step; subst.
+      + admit.
+      + eapply PAR.
+        * eapply IHWT1.
+          admit. (* Need new lemma *)
+          assumption.
+        * eapply IHWT2.
+          admit. (* Need new lemma *)
+          admit.
+
+End runtime_props.
